basic_topology/Net.lean
@@ -32,6 +32,8 @@ def net_converges {X: Type u} {Δ: Type v} (T: Family X) (R: Relation Δ Δ) (a:
 def neighborhood_direction (T: Family X) (x: X): Endorelation (Nbhds T x) :=
   fun N₁ N₂ => N₂.val ⊆ N₁.val
 
+--dfn a sequence is a net --
+
 theorem neighborhood_direction_directed_set (T: Family X) (x: X) (hT: IsTopology T): directed (neighborhood_direction T x) := by
   repeat constructor
   · intro Nx
